coq/LLVMGen/Compiler.v
@@ -1095,3 +1095,179 @@ Definition LLVMGen
                        ]
        ).
 
+Record FSHCOLProgram :=
+  mkFSHCOLProgram
+    {
+      i: nat;
+      o: nat;
+      name: string;
+      globals: list (string * FSHValType) ;
+      op: DSHOperator;
+    }.
+
+(* To move to Utils? *)
+Definition rotate {A:Type} (default:A) (lst:list (A)): (A*(list A))
+  := match lst with
+     | [] => (default,[])
+     | (x::xs) => (x,app xs [x])
+     end.
+
+Fixpoint constList
+         (len: nat)
+         (data:list binary64) :
+  ((list binary64) * (list binary64))
+  :=
+    match len with
+    | O => (data,[])
+    | S len' => let '(x, data') := rotate Float64Zero data in
+               let '(data'',res) := constList len' data' in
+               (data'', x :: res)
+    end.
+
+Definition constArray
+           (len: nat)
+           (data:list binary64)
+  : ((list binary64)*(list (texp typ)))
+  :=  let (data, l) := constList len data in
+      (data,List.map (fun x => (TYPE_Double, genFloatV x)) l).
+
+Definition constMemBlock
+         (len: nat)
+         (data:list binary64)
+  : ((list binary64)*mem_block)
+  := let (data, l) := constList len data in
+     (data, mem_block_of_list l).
+
+Fixpoint initIRGlobals
+         (data: list binary64)
+         (x: list (string * FSHValType))
+  : err (list binary64 * list (toplevel_entity typ (list (block typ))))
+  :=
+    match x with
+    | nil => ret (data,[])
+    | cons (nm, t) xs =>
+      '(data,gs) <- initIRGlobals data xs ;;
+      match t with
+      | FSHnatValType => raise "FSHnatValType global type not supported"
+      | FSHFloatValType =>
+        let '(x, data) := rotate Float64Zero data in
+        ret (data, TLE_Global {|
+                   g_ident        := Name nm;
+                   g_typ          := getIRType t ;
+                   g_constant     := true ;
+                   g_exp          := Some (EXP_Double x);
+                   g_linkage      := Some LINKAGE_Internal ;
+                   g_visibility   := None ;
+                   g_dll_storage  := None ;
+                   g_thread_local := None ;
+                   g_unnamed_addr := true ;
+                   g_addrspace    := None ;
+                   g_externally_initialized := false ;
+                   g_section      := None ;
+                   g_align        := None ; (* TODO: maybe need to alight to 64-bit boundary? *)
+                 |} :: gs)
+      | FSHvecValType n =>
+        let (data, arr) := constArray n data in
+        ret (data, TLE_Global {|
+                   g_ident        := Name nm;
+                   g_typ          := getIRType t ;
+                   g_constant     := true ;
+                   g_exp          := Some (EXP_Array arr);
+                   g_linkage      := Some LINKAGE_Internal ;
+                   g_visibility   := None ;
+                   g_dll_storage  := None ;
+                   g_thread_local := None ;
+                   g_unnamed_addr := true ;
+                   g_addrspace    := None ;
+                   g_externally_initialized := false ;
+                   g_section      := None ;
+                   g_align        := Some Utils.PtrAlignment ;
+                 |} :: gs)
+      end
+    end.
+
+Definition genMain
+           (i o: nat)
+           (op_name: string)
+           (globals: list (string * FSHValType))
+           (data:list binary64)
+  :
+    LLVMAst.toplevel_entities _ (list (LLVMAst.block typ)) :=
+  let x := Name "X" in
+  let xtyp := getIRType (FSHvecValType i) in
+  let xptyp := TYPE_Pointer xtyp in
+  let '(_,xdata) := constArray i data in
+  let y := Name "Y" in
+  let ytyp := getIRType (FSHvecValType o) in
+  let yptyp := TYPE_Pointer ytyp in
+  let ftyp := TYPE_Function TYPE_Void [xptyp; yptyp] in
+  let z := Name "z" in
+  [
+    TLE_Comment " X data" ;
+      TLE_Global
+        {|
+          g_ident        := x;
+          g_typ          := xtyp;
+          g_constant     := true;
+          g_exp          := Some (EXP_Array xdata);
+          g_linkage      := None;
+          g_visibility   := None;
+          g_dll_storage  := None;
+          g_thread_local := None;
+          g_unnamed_addr := false;
+          g_addrspace    := None;
+          g_externally_initialized := false;
+          g_section      := None;
+          g_align        := None;
+        |} ;
+      TLE_Comment " Main function" ;
+      TLE_Definition
+        {|
+          df_prototype   :=
+            {|
+              dc_name        := Name ("main") ;
+              dc_type        := TYPE_Function ytyp [] ;
+              dc_param_attrs := ([],
+                                 []);
+              dc_linkage     := None ;
+              dc_visibility  := None ;
+              dc_dll_storage := None ;
+              dc_cconv       := None ;
+              dc_attrs       := []   ;
+              dc_section     := None ;
+              dc_align       := None ;
+              dc_gc          := None
+            |} ;
+          df_args        := [];
+          df_instrs      := [
+                             {|
+                               blk_id    := Name "main_block" ;
+                               blk_phis  := [];
+                               blk_code  :=
+                                 List.app (allocTempArrayCode y o)
+                                          [
+                                            (IVoid 0%Z, INSTR_Call (TYPE_Void, EXP_Ident (ID_Global (Name op_name))) [(xptyp, EXP_Ident (ID_Global x)); (yptyp, EXP_Ident (ID_Local y))]) ;
+                                              (IId z, INSTR_Load false ytyp (yptyp, EXP_Ident (ID_Local y)) None )
+                                          ]
+                               ;
+
+                               blk_term  := (IId (Name "main_ret"), TERM_Ret (ytyp, EXP_Ident (ID_Local z))) ;
+                               blk_comments := None
+                             |}
+
+                           ]
+        |}].
+
+Definition compile (p: FSHCOLProgram): list binary64 -> err (toplevel_entities typ (list (block typ))) :=
+  match p return (list binary64 -> _) with
+  | mkFSHCOLProgram i o name globals op =>
+    fun data' =>
+      '(data'',ginit) <- initIRGlobals data' globals ;;
+       let ginit := app [TLE_Comment "Global variables"] ginit in
+       let main := genMain i o name globals data'' in
+       prog <- LLVMGen i o globals false op name ;;
+       let code := app (app ginit prog) main in
+       ret code
+  end.
+
+
