coq/LLVMGen/Correctness.v
@@ -1,0 +1,96 @@
+Require Import Coq.Strings.String.
+Require Import Coq.Lists.List.
+Require Import Coq.Numbers.BinNums. (* for Z scope *)
+Require Import Coq.ZArith.BinInt.
+
+Require Import Helix.FSigmaHCOL.FSigmaHCOL.
+Require Import Helix.DSigmaHCOL.DSigmaHCOLITree.
+Require Import Helix.LLVMGen.Compiler.
+Require Import Helix.LLVMGen.Externals.
+Require Import Helix.Util.ErrorSetoid.
+
+Require Import Vellvm.Numeric.Fappli_IEEE_extra.
+Require Import Vellvm.LLVMEvents.
+Require Import Vellvm.Denotation.
+Require Import Vellvm.Handlers.Memory.
+Require Import Vellvm.TopLevel.
+Require Import Vellvm.LLVMAst.
+Require Import Vellvm.CFG.
+Require Import Vellvm.TopLevelRefinements.
+
+Require Import ITree.ITree.
+Require Import ITree.Basics.Basics.
+
+Require Import Flocq.IEEE754.Binary.
+Require Import Flocq.IEEE754.Bits.
+
+Require Import ExtLib.Structures.Monads.
+
+
+Set Implicit Arguments.
+Set Strict Implicit.
+
+Import MDSHCOLOnFloat64.
+
+Definition model_llvm' := model_to_L3 helix_intrinsics.
+
+Definition E: Type -> Type := (StaticFailE +' DynamicFailE) +' (IO.CallE +' IO.PickE +' UBE +' DebugE +' FailureE).
+
+Definition model_llvm p: itree E _ := translate (@subevent _ E _) (model_llvm' p).
+
+Import ListNotations.
+Import MonadNotation.
+Local Open Scope monad_scope.
+
+Fixpoint denote_initFSHGlobals
+         (data: list binary64)
+         (globals: list (string * FSHValType))
+  : itree Event (list binary64 * evalContext) :=
+    match globals with
+    | [] => ret (data, [])
+    | (_,gt)::gs =>
+      match gt with
+      | FSHnatValType => Sfail "Unsupported global type: nat"
+      | FSHFloatValType =>
+        '(data,σ) <- denote_initFSHGlobals data gs ;;
+         let '(x, data) := rotate Float64Zero data in
+         ret (data, (DSHCTypeVal x)::σ)
+      | FSHvecValType n =>
+        '(data,σ) <- denote_initFSHGlobals data gs ;;
+         let (data,mb) := constMemBlock n data in
+         k <- trigger (MemAlloc n);;
+         trigger (MemSet k mb);;
+         let p := DSHPtrVal k in
+         ret (data, (p::σ))
+      end
+    end.
+
+(* Definition denote_FSHCOL (t:FSHCOLProgram) (data:list binary64) *)
+(*   : itree (StaticFailE +' DynamicFailE) (list binary64) := *)
+(*   xindex <- trigger (MemAlloc xindex mem_empty);; *)
+(*   yindex <- trigger (MemAlloc yindex mem_empty);; *)
+(*   '(data, σ) <- initFSHGlobals data mem globals ;; *)
+(*   let '(data, x) := constMemBlock i data in *)
+(*   let mem := memory_set mem xindex x in *)
+(*   let σ := List.app σ [DSHPtrVal yindex; DSHPtrVal xindex] in *)
+(*   match evalDSHOperator σ op mem (estimateFuel op) with *)
+(*   | Some (inr mem) => *)
+(*     yb <- trywith "No output memory block" (memory_lookup mem yindex) ;; *)
+(*        mem_to_list "Invalid output memory block" o yb *)
+(*   | Some (inl msg) => inl msg *)
+(*   | None => raise "evalDSHOperator returns None" *)
+(*   end. *)
+
+
+
+(* Theorem compiler_correct: *)
+(*   forall (i o: nat) *)
+(*     (globals: list (string*FSHValType)) *)
+(*     (globals_extern: bool) *)
+(*     (fshcol: DSHOperator) *)
+(*     (funname: string) *)
+(*     p σ mem, *)
+(*   exists RR, *)
+(*     LLVMGen i o globals globals_extern fshcol funname ≡ inr p -> *)
+(*     eutt RR (denoteDSHOperator σ fshcol mem) (model_user ). *)
+
