coq/LLVMGen/Tests.v
@@ -160,159 +160,6 @@ Import MonadNotation.
 Import IO.
 Export IO.DV.
 
-Definition rotate {A:Type} (default:A) (lst:list (A)): (A*(list A))
-  := match lst with
-     | [] => (default,[])
-     | (x::xs) => (x,app xs [x])
-     end.
-
-
-Fixpoint constList
-         (len: nat)
-         (data:list binary64) :
-  ((list binary64) * (list binary64))
-  :=
-    match len with
-    | O => (data,[])
-    | S len' => let '(x, data') := rotate Float64Zero data in
-               let '(data'',res) := constList len' data' in
-               (data'', x :: res)
-    end.
-
-Definition constArray
-           (len: nat)
-           (data:list binary64)
-  : ((list binary64)*(list (texp typ)))
-  :=  let (data, l) := constList len data in
-      (data,List.map (fun x => (TYPE_Double, genFloatV x)) l).
-
-Definition constMemBlock
-         (len: nat)
-         (data:list binary64)
-  : ((list binary64)*mem_block)
-  := let (data, l) := constList len data in
-     (data, mem_block_of_list l).
-
-Fixpoint initIRGlobals
-         (data: list binary64)
-         (x: list (string * FSHValType))
-  : err (list binary64 * list (toplevel_entity typ (list (block typ))))
-  :=
-    match x with
-    | nil => ret (data,[])
-    | cons (nm, t) xs =>
-      '(data,gs) <- initIRGlobals data xs ;;
-      match t with
-      | FSHnatValType => raise "FSHnatValType global type not supported"
-      | FSHFloatValType =>
-        let '(x, data) := rotate Float64Zero data in
-        ret (data, TLE_Global {|
-                   g_ident        := Name nm;
-                   g_typ          := getIRType t ;
-                   g_constant     := true ;
-                   g_exp          := Some (EXP_Double x);
-                   g_linkage      := Some LINKAGE_Internal ;
-                   g_visibility   := None ;
-                   g_dll_storage  := None ;
-                   g_thread_local := None ;
-                   g_unnamed_addr := true ;
-                   g_addrspace    := None ;
-                   g_externally_initialized := false ;
-                   g_section      := None ;
-                   g_align        := None ; (* TODO: maybe need to alight to 64-bit boundary? *)
-                 |} :: gs)
-      | FSHvecValType n =>
-        let (data, arr) := constArray n data in
-        ret (data, TLE_Global {|
-                   g_ident        := Name nm;
-                   g_typ          := getIRType t ;
-                   g_constant     := true ;
-                   g_exp          := Some (EXP_Array arr);
-                   g_linkage      := Some LINKAGE_Internal ;
-                   g_visibility   := None ;
-                   g_dll_storage  := None ;
-                   g_thread_local := None ;
-                   g_unnamed_addr := true ;
-                   g_addrspace    := None ;
-                   g_externally_initialized := false ;
-                   g_section      := None ;
-                   g_align        := Some Utils.PtrAlignment ;
-                 |} :: gs)
-      end
-    end.
-
-Definition genMain
-           (i o: nat)
-           (op_name: string)
-           (globals: list (string * FSHValType))
-           (data:list binary64)
-  :
-    LLVMAst.toplevel_entities _ (list (LLVMAst.block typ)) :=
-  let x := Name "X" in
-  let xtyp := getIRType (FSHvecValType i) in
-  let xptyp := TYPE_Pointer xtyp in
-  let '(_,xdata) := constArray i data in
-  let y := Name "Y" in
-  let ytyp := getIRType (FSHvecValType o) in
-  let yptyp := TYPE_Pointer ytyp in
-  let ftyp := TYPE_Function TYPE_Void [xptyp; yptyp] in
-  let z := Name "z" in
-  [
-    TLE_Comment " X data" ;
-      TLE_Global
-        {|
-          g_ident        := x;
-          g_typ          := xtyp;
-          g_constant     := true;
-          g_exp          := Some (EXP_Array xdata);
-          g_linkage      := None;
-          g_visibility   := None;
-          g_dll_storage  := None;
-          g_thread_local := None;
-          g_unnamed_addr := false;
-          g_addrspace    := None;
-          g_externally_initialized := false;
-          g_section      := None;
-          g_align        := None;
-        |} ;
-      TLE_Comment " Main function" ;
-      TLE_Definition
-        {|
-          df_prototype   :=
-            {|
-              dc_name        := Name ("main") ;
-              dc_type        := TYPE_Function ytyp [] ;
-              dc_param_attrs := ([],
-                                 []);
-              dc_linkage     := None ;
-              dc_visibility  := None ;
-              dc_dll_storage := None ;
-              dc_cconv       := None ;
-              dc_attrs       := []   ;
-              dc_section     := None ;
-              dc_align       := None ;
-              dc_gc          := None
-            |} ;
-          df_args        := [];
-          df_instrs      := [
-                             {|
-                               blk_id    := Name "main_block" ;
-                               blk_phis  := [];
-                               blk_code  :=
-                                 List.app (allocTempArrayCode y o)
-                                          [
-                                            (IVoid 0, INSTR_Call (TYPE_Void, EXP_Ident (ID_Global (Name op_name))) [(xptyp, EXP_Ident (ID_Global x)); (yptyp, EXP_Ident (ID_Local y))]) ;
-                                              (IId z, INSTR_Load false ytyp (yptyp, EXP_Ident (ID_Local y)) None )
-                                          ]
-                               ;
-
-                               blk_term  := (IId (Name "main_ret"), TERM_Ret (ytyp, EXP_Ident (ID_Local z))) ;
-                               blk_comments := None
-                             |}
-
-                           ]
-        |}].
-
 Definition test_interpreter := TopLevelEnv.interpreter_user helix_intrinsics.
 
 
@@ -373,6 +220,34 @@ Fixpoint initFSHGlobals
                   end
     end.
 
+(* Definition evalFSHCOLOperator *)
+(*            (i o: nat) *)
+(*            (name: string) *)
+(*            (globals: list (string * FSHValType)) *)
+(*            (op: DSHOperator) *)
+(*            (data:list binary64) *)
+(*   : err (list binary64) *)
+(*   := *)
+(*     let mem := memory_empty in *)
+(*     let xindex := 1%nat in *)
+(*     let yindex := 0%nat in *)
+(*     let mem := memory_set mem xindex mem_empty in (* placeholder *) *)
+(*     let mem := memory_set mem yindex mem_empty in *)
+(*     '(mem, data, σ) <- initFSHGlobals data mem globals ;; *)
+(*      let '(data, x) := constMemBlock i data in *)
+(*      let xindex := 1%nat in *)
+(*      let yindex := 0%nat in *)
+(*      let mem := memory_set mem xindex x in *)
+(*      let σ := List.app σ [DSHPtrVal yindex; DSHPtrVal xindex] in *)
+(*      match evalDSHOperator σ op mem (estimateFuel op) with *)
+(*      | Some (inr mem) => *)
+(*        yb <- trywith "No output memory block" (memory_lookup mem yindex) ;; *)
+(*           mem_to_list "Invalid output memory block" o yb *)
+(*      | Some (inl msg) => inl msg *)
+(*      | None => raise "evalDSHOperator returns None" *)
+(*      end. *)
+
+
 Definition evalFSHCOLOperator
            (i o: nat)
            (name: string)
@@ -381,16 +256,17 @@ Definition evalFSHCOLOperator
            (data:list binary64)
   : err (list binary64)
   :=
+
     let mem := memory_empty in
-    let xindex := 1%nat in
-    let yindex := 0%nat in
-    let mem := memory_set mem xindex mem_empty in (* placeholder *)
-    let mem := memory_set mem yindex mem_empty in
+    (* Initializes the input address *)
     '(mem, data, σ) <- initFSHGlobals data mem globals ;;
-     let '(data, x) := constMemBlock i data in
-     let xindex := 1%nat in
-     let yindex := 0%nat in
-     let mem := memory_set mem xindex x in
+    let xindex := memory_new mem in
+    let '(data, x) := constMemBlock i data in
+    let mem := memory_set mem xindex x in
+    (* Initializes the output address *)
+    let yindex :=  memory_new mem in
+    let mem := memory_set mem yindex mem_empty in
+
      let σ := List.app σ [DSHPtrVal yindex; DSHPtrVal xindex] in
      match evalDSHOperator σ op mem (estimateFuel op) with
      | Some (inr mem) =>
